src/EvarsFacts.v
@@ -1,0 +1,91 @@
+(******************************************************************************)
+(* pose_facts facts                                                           *)
+(* prove_later facts                                                          *)
+(* close_facts                                                                *)
+(******************************************************************************)
+
+Definition close_facts P1 P2 :=
+  P2 -> P1.
+
+Lemma pose_facts_lemma :
+  forall facts facts_closed P, (facts -> P) -> close_facts facts facts_closed -> facts_closed -> P.
+Proof. unfold close_facts. tauto. Qed.
+
+Ltac pose_facts facts :=
+  eapply pose_facts_lemma; [ intro facts | .. ].
+
+Ltac closed_facts_ty T :=
+  lazymatch T with
+  | and ?x ?y =>
+    lazymatch y with
+    | and _ _ =>
+      let y' := closed_facts_ty y in
+      constr:(and x y')
+    | _ => constr:(x)
+    end
+  end.
+
+Ltac close_facts_aux tm ty :=
+  lazymatch ty with
+  | and ?x ?y =>
+    split; [apply (@proj1 x y tm) | close_facts_aux (@proj2 x y tm) y]
+  | ?x => split; [apply tm | exact I]
+  end.
+
+Ltac close_facts :=
+  unfold close_facts;
+  let facts_closed := fresh "facts_closed" in
+  intro facts_closed;
+  match goal with
+  | |- ?facts =>
+    let facts_closed_T := closed_facts_ty facts in
+    close_facts_aux facts_closed facts_closed_T
+  end.
+
+Ltac nested_and_proj2 p :=
+  lazymatch p with
+  | and _ ?y => nested_and_proj2 y
+  | ?x => x
+  end.
+
+Ltac add_fact P facts :=
+  let T := type of facts in
+  let TE := nested_and_proj2 T in
+  let TE' := fresh in
+  evar (TE' : Prop);
+  unify TE (and P TE');
+  subst TE'.
+
+Ltac apply_last_fact_aux tm ty :=
+  lazymatch ty with
+  | and ?x ?y =>
+    lazymatch y with
+    | and _ _ => apply_last_fact_aux (@proj2 x y tm) y
+    | _ =>
+      apply (@proj1 x y tm)
+    end
+  end.
+
+Ltac apply_last_fact facts :=
+  let T := type of facts in
+  apply_last_fact_aux facts T.
+
+Ltac prove_later facts :=
+  match goal with
+    |- ?P => add_fact P facts
+  end;
+  simpl in facts;
+  apply_last_fact facts.
+
+Goal True.
+  pose_facts facts.
+
+  assert (H1 : 1 + 1 = 2) by (prove_later facts).
+  assert (H2 : 1 + 2 = 3) by (prove_later facts).
+  assert (H3 : 1 + 3 = 4) by (prove_later facts).
+
+  tauto.
+  close_facts.
+
+  repeat split; reflexivity.
+Qed.
